F_mu_ref_par/fundamental_binary.v
@@ -8,18 +8,15 @@ Section bin_log_def.
   Notation D := (prodC valC valC -n> iPropG lang Σ).
 
   Definition bin_log_related (Δ : listC D) (Γ : list type)
-      (e e' : expr) (τ : type) : Prop := ∀ vvs ρ j K,
-    length Γ = length vvs →
-    heapI_ctx ★ spec_ctx ρ ★ [∧] zip_with (λ τ, interp τ Δ) Γ vvs ★
-      j ⤇ fill K (e'.[env_subst (vvs.*2)])
-    ⊢ WP e.[env_subst (vvs.*1)] {{ v, ∃ v',
-        j ⤇ fill K (# v') ★ interp τ Δ (v, v') }}.
+      (e e' : expr) (τ : type) : Prop := ∀ vvs ρ,
+    heapI_ctx ∧ spec_ctx ρ ∧
+    ⟦ Γ ⟧* Δ vvs ⊢ ⟦ τ ⟧ₑ Δ (e.[env_subst (vvs.*1)], e'.[env_subst (vvs.*2)]).
 End bin_log_def.
 
 Notation "Δ ∥ Γ ⊨ e '≤log≤' e' : τ" :=
   (bin_log_related Δ Γ e e' τ) (at level 74, Γ, e, e', τ at next level).
 
-Section typed_interp.
+Section fundamental.
   Context `{heapIG Σ, cfgSG Σ}.
   Notation D := (prodC valC valC -n> iPropG lang Σ).
   Implicit Types e : expr.
@@ -37,67 +34,105 @@ Section typed_interp.
 
   Local Ltac value_case := iApply wp_value; [cbn; rewrite ?to_of_val; trivial|].
 
-  Notation "✓✓ Δ" := (ctx_PersistentP Δ) (at level 20).
+  (* Put all quantifiers at the outer level *)
+  Lemma bin_log_related_alt {Δ Γ e e' τ} :
+    Δ ∥ Γ ⊨ e ≤log≤ e' : τ → ∀ vvs ρ j K,
+    heapI_ctx ★ spec_ctx ρ ★ ⟦ Γ ⟧* Δ vvs ★ j ⤇ fill K (e'.[env_subst (vvs.*2)])
+    ⊢ WP e.[env_subst (vvs.*1)] {{ v, ∃ v',
+        j ⤇ fill K (# v') ★ interp τ Δ (v, v') }}.
+  Proof.
+    iIntros {Hlog vvs ρ j K} "(#Hh & #Hs & HΓ & Hj)".
+    iApply (Hlog with "[HΓ] *"); iFrame; eauto.
+  Qed.
 
-  Lemma typed_binary_interp_Pair Δ Γ e1 e2 e1' e2' τ1 τ2 {HΔ : ✓✓ Δ}
+  Notation "' H" := (bin_log_related_alt H) (at level 8).
+  Notation "✓ₚ Δ" := (env_PersistentP Δ) (at level 20).
+
+  Lemma bin_log_related_Var Δ Γ x τ {HΔ : ✓ₚ Δ} :
+    Γ !! x = Some τ → Δ ∥ Γ ⊨ Var x ≤log≤ Var x : τ.
+  Proof.
+    iIntros {? vvs ρ} "#(Hh & Hs & HΓ)"; iIntros {j K} "Hj /=".
+    iDestruct (interp_env_Some_l with "HΓ") as { [v v'] } "[% ?]"; first done.
+    rewrite /env_subst !list_lookup_fmap; simplify_option_eq. value_case; eauto.
+  Qed.
+
+  Lemma bin_log_related_Unit Δ Γ {HΔ: ✓ₚ Δ} : Δ ∥ Γ ⊨ Unit ≤log≤ Unit : TUnit.
+  Proof.
+    iIntros {vvs ρ} "#(Hh & Hs & HΓ)"; iIntros {j K} "Hj /=".
+    value_case. iExists UnitV; eauto.
+  Qed.
+
+  Lemma bin_log_related_Nat Δ Γ n {HΔ: ✓ₚ Δ} : Δ ∥ Γ ⊨ ♯ n ≤log≤ ♯ n : TNat.
+  Proof.
+    iIntros {vvs ρ} "#(Hh & Hs & HΓ)"; iIntros {j K} "Hj /=".
+    value_case. iExists (♯v _); eauto.
+  Qed.
+
+  Lemma bin_log_related_Bool Δ Γ b {HΔ: ✓ₚ Δ} : Δ ∥ Γ ⊨ ♭ b ≤log≤ ♭ b : TBool.
+  Proof.
+    iIntros {vvs ρ} "#(Hh & Hs & HΓ)"; iIntros {j K} "Hj /=".
+    value_case. iExists (♭v _); eauto.
+  Qed.
+
+  Lemma bin_log_related_Pair Δ Γ e1 e2 e1' e2' τ1 τ2 {HΔ : ✓ₚ Δ}
       (IHHtyped1 : Δ ∥ Γ ⊨ e1 ≤log≤ e1' : τ1)
       (IHHtyped2 : Δ ∥ Γ ⊨ e2 ≤log≤ e2' : τ2) :
     Δ ∥ Γ ⊨ Pair e1 e2 ≤log≤ Pair e1' e2' : TProd τ1 τ2.
   Proof.
-    iIntros {vvs ρ j K Hlen} "(#Hh & #Hs & #HΓ & Hj) /=".
+    iIntros {vvs ρ} "#(Hh & Hs & HΓ)"; iIntros {j K} "Hj /=".
     smart_wp_bind (PairLCtx e2.[env_subst _]) v v' "[Hv #Hiv]"
-      (IHHtyped1 _ _ j (K ++ [PairLCtx e2'.[env_subst _] ])).
+      ('IHHtyped1 _ _ j (K ++ [PairLCtx e2'.[env_subst _] ])).
     smart_wp_bind (PairRCtx v) w w' "[Hw #Hiw]"
-      (IHHtyped2 _ _ j (K ++ [PairRCtx v'])).
+      ('IHHtyped2 _ _ j (K ++ [PairRCtx v'])).
     value_case. iExists (PairV v' w'); iFrame "Hw".
     iExists (v, v'), (w, w'); simpl; repeat iSplit; trivial.
   Qed.
 
-  Lemma typed_binary_interp_Fst Δ Γ e e' τ1 τ2 {HΔ : ✓✓ Δ}
+  Lemma bin_log_related_Fst Δ Γ e e' τ1 τ2 {HΔ : ✓ₚ Δ}
       (IHHtyped : Δ ∥ Γ ⊨ e ≤log≤ e' : TProd τ1 τ2) :
     Δ ∥ Γ ⊨ Fst e ≤log≤ Fst e' : τ1.
   Proof.
-    iIntros {vvs ρ j K Hlen} "(#Hh & #Hs & #HΓ & Hj) /=".
-    smart_wp_bind (FstCtx) v v' "[Hv #Hiv]" (IHHtyped _ _ j (K ++ [FstCtx])); cbn.
+    iIntros {vvs ρ} "#(Hh & Hs & HΓ)"; iIntros {j K} "Hj /=".
+    smart_wp_bind (FstCtx) v v' "[Hv #Hiv]" ('IHHtyped _ _ j (K ++ [FstCtx])); cbn.
     iDestruct "Hiv" as { [w1 w1'] [w2 w2'] } "#[% [Hw1 Hw2]]"; simplify_eq.
     iPvs (step_fst _ _ j K (# w1') w1' (# w2') w2' with "* [-]") as "Hw"; eauto.
     iApply wp_fst; eauto.
   Qed.
 
-  Lemma typed_binary_interp_Snd Δ Γ e e' τ1 τ2 {HΔ : ✓✓ Δ}
+  Lemma bin_log_related_Snd Δ Γ e e' τ1 τ2 {HΔ : ✓ₚ Δ}
       (IHHtyped : Δ ∥ Γ ⊨ e ≤log≤ e' : TProd τ1 τ2) :
     Δ ∥ Γ ⊨ Snd e ≤log≤ Snd e' : τ2.
   Proof.
-    iIntros {vvs ρ j K Hlen} "(#Hh & #Hs & #HΓ & Hj) /=".
-    smart_wp_bind (SndCtx) v v' "[Hv #Hiv]" (IHHtyped _ _ j (K ++ [SndCtx])); cbn.
+    iIntros {vvs ρ} "#(Hh & Hs & HΓ)"; iIntros {j K} "Hj /=".
+    smart_wp_bind (SndCtx) v v' "[Hv #Hiv]" ('IHHtyped _ _ j (K ++ [SndCtx])); cbn.
     iDestruct "Hiv" as { [w1 w1'] [w2 w2'] } "#[% [Hw1 Hw2]]"; simplify_eq.
     iPvs (step_snd _ _ j K (# w1') w1' (# w2') w2' with "* [-]") as "Hw"; eauto.
     iApply wp_snd; eauto.
   Qed.
 
-  Lemma typed_binary_interp_InjL Δ Γ e e' τ1 τ2 {HΔ : ✓✓ Δ}
+  Lemma bin_log_related_InjL Δ Γ e e' τ1 τ2 {HΔ : ✓ₚ Δ}
       (IHHtyped : Δ ∥ Γ ⊨ e ≤log≤ e' : τ1) :
     Δ ∥ Γ ⊨ InjL e ≤log≤ InjL e' : (TSum τ1 τ2).
   Proof.
-    iIntros {vvs ρ j K Hlen} "(#Hh & #Hs & #HΓ & Hj) /=".
+    iIntros {vvs ρ} "#(Hh & Hs & HΓ)"; iIntros {j K} "Hj /=".
     smart_wp_bind (InjLCtx) v v' "[Hv #Hiv]"
-      (IHHtyped _ _ j (K ++ [InjLCtx])); cbn.
+      ('IHHtyped _ _ j (K ++ [InjLCtx])); cbn.
     value_case. iExists (InjLV v'); iFrame "Hv".
     iLeft; iExists (_,_); eauto 10.
   Qed.
 
-  Lemma typed_binary_interp_InjR Δ Γ e e' τ1 τ2 {HΔ : ✓✓ Δ}
+  Lemma bin_log_related_InjR Δ Γ e e' τ1 τ2 {HΔ : ✓ₚ Δ}
       (IHHtyped : Δ ∥ Γ ⊨ e ≤log≤ e' : τ2) :
     Δ ∥ Γ ⊨ InjR e ≤log≤ InjR e' : TSum τ1 τ2.
   Proof.
-    iIntros {vvs ρ j K Hlen} "(#Hh & #Hs & #HΓ & Hj) /=".
+    iIntros {vvs ρ} "#(Hh & Hs & HΓ)"; iIntros {j K} "Hj /=".
     smart_wp_bind (InjRCtx) v v' "[Hv #Hiv]"
-      (IHHtyped _ _ j (K ++ [InjRCtx])); cbn.
+      ('IHHtyped _ _ j (K ++ [InjRCtx])); cbn.
     value_case. iExists (InjRV v'); iFrame "Hv".
     iRight; iExists (_,_); eauto 10.
   Qed.
 
-  Lemma typed_binary_interp_Case Δ Γ e0 e1 e2 e0' e1' e2' τ1 τ2 τ3 {HΔ : ✓✓ Δ}
+  Lemma bin_log_related_Case Δ Γ e0 e1 e2 e0' e1' e2' τ1 τ2 τ3 {HΔ : ✓ₚ Δ}
       (Hclosed2 : ∀ f, e1.[iter (S (length Γ)) up f] = e1)
       (Hclosed3 : ∀ f, e2.[iter (S (length Γ)) up f] = e2)
       (Hclosed2' : ∀ f, e1'.[iter (S (length Γ)) up f] = e1')
@@ -107,52 +142,51 @@ Section typed_interp.
       (IHHtyped3 : Δ ∥ τ2 :: Γ ⊨ e2 ≤log≤ e2' : τ3) :
     Δ ∥ Γ ⊨ Case e0 e1 e2 ≤log≤ Case e0' e1' e2' : τ3.
   Proof.
-    iIntros {vvs ρ j K Hlen} "(#Hh & #Hs & #HΓ & Hj) /=".
+    iIntros {vvs ρ} "#(Hh & Hs & HΓ)"; iIntros {j K} "Hj /=".
+    iDestruct (interp_env_length with "HΓ") as %?.
     smart_wp_bind (CaseCtx _ _) v v' "[Hv #Hiv]"
-      (IHHtyped1 _ _ j (K ++ [CaseCtx _ _])); cbn.
+      ('IHHtyped1 _ _ j (K ++ [CaseCtx _ _])); cbn.
     iDestruct "Hiv" as "[Hiv|Hiv]".
     - iDestruct "Hiv" as { [w w'] } "[% Hw]"; simplify_eq.
       iPvs (step_case_inl _ _ j K (# w') w' with "* [-]") as "Hz"; eauto.
-      iApply wp_case_inl; auto 1 using to_of_val; asimpl.
-      specialize (IHHtyped2 ((w,w') :: vvs)); cbn in IHHtyped2.
-      erewrite <- ?n_closed_subst_head_simpl in IHHtyped2; eauto;
-        simpl; try rewrite fmap_length; eauto with f_equal.
-      iNext. iApply IHHtyped2; eauto.
+      iApply wp_case_inl; auto 1 using to_of_val. iNext.
+      asimpl. erewrite !n_closed_subst_head_simpl by (rewrite ?fmap_length; eauto).
+      iApply ('IHHtyped2 ((w,w') :: vvs)); repeat iSplit; eauto.
+      iApply interp_env_cons; auto.
     - iDestruct "Hiv" as { [w w'] } "[% Hw]"; simplify_eq.
       iPvs (step_case_inr _ _ j K (# w') w' with "* [-]") as "Hz"; eauto.
-      iApply wp_case_inr; auto 1 using to_of_val; asimpl.
-      specialize (IHHtyped3 ((w,w') :: vvs)); cbn in IHHtyped3.
-      erewrite <- ?n_closed_subst_head_simpl in IHHtyped3; eauto;
-        simpl; try rewrite map_length; eauto with f_equal.
-      iNext. iApply IHHtyped3; eauto 10.
+      iApply wp_case_inr; auto 1 using to_of_val. iNext.
+      asimpl. erewrite !n_closed_subst_head_simpl by (rewrite ?fmap_length; eauto).
+      iApply ('IHHtyped3 ((w,w') :: vvs)); repeat iSplit; eauto.
+      iApply interp_env_cons; auto.
   Qed.
 
-  Lemma typed_binary_interp_If Δ Γ e0 e1 e2 e0' e1' e2' τ {HΔ : ✓✓ Δ}
+  Lemma bin_log_related_If Δ Γ e0 e1 e2 e0' e1' e2' τ {HΔ : ✓ₚ Δ}
       (IHHtyped1 : Δ ∥ Γ ⊨ e0 ≤log≤ e0' : TBool)
       (IHHtyped2 : Δ ∥ Γ ⊨ e1 ≤log≤ e1' : τ)
       (IHHtyped3 : Δ ∥ Γ ⊨ e2 ≤log≤ e2' : τ) :
     Δ ∥ Γ ⊨ If e0 e1 e2 ≤log≤ If e0' e1' e2' : τ.
   Proof.
-    iIntros {vvs ρ j K Hlen} "(#Hh & #Hs & #HΓ & Hj) /=".
+    iIntros {vvs ρ} "#(Hh & Hs & HΓ)"; iIntros {j K} "Hj /=".
     smart_wp_bind (IfCtx _ _) v v' "[Hv #Hiv]"
-      (IHHtyped1 _ _ j (K ++ [IfCtx _ _])); cbn.
+      ('IHHtyped1 _ _ j (K ++ [IfCtx _ _])); cbn.
     iDestruct "Hiv" as { [] } "[% %]"; simplify_eq/=.
     - iPvs (step_if_true _ _ j K with "* [-]") as "Hz"; eauto.
-      iApply wp_if_true. iNext. iApply IHHtyped2; eauto.
+      iApply wp_if_true. iNext. iApply 'IHHtyped2; eauto.
     - iPvs (step_if_false _ _ j K with "* [-]") as "Hz"; eauto.
-      iApply wp_if_false. iNext. iApply IHHtyped3; eauto.
+      iApply wp_if_false. iNext. iApply 'IHHtyped3; eauto.
   Qed.
 
-  Lemma typed_binary_interp_nat_bin_op Δ Γ op e1 e2 e1' e2' {HΔ : ✓✓ Δ}
+  Lemma bin_log_related_nat_bin_op Δ Γ op e1 e2 e1' e2' {HΔ : ✓ₚ Δ}
       (IHHtyped1 : Δ ∥ Γ ⊨ e1 ≤log≤ e1' : TNat)
       (IHHtyped2 : Δ ∥ Γ ⊨ e2 ≤log≤ e2' : TNat) :
     Δ ∥ Γ ⊨ BinOp op e1 e2 ≤log≤ BinOp op e1' e2' : binop_res_type op.
   Proof.
-    iIntros {vvs ρ j K Hlen} "(#Hh & #Hs & #HΓ & Hj) /=".
+    iIntros {vvs ρ} "#(Hh & Hs & HΓ)"; iIntros {j K} "Hj /=".
     smart_wp_bind (BinOpLCtx _ _) v v' "[Hv #Hiv]"
-                  (IHHtyped1 _ _ j (K ++ [BinOpLCtx _ _])); cbn.
+                  ('IHHtyped1 _ _ j (K ++ [BinOpLCtx _ _])); cbn.
     smart_wp_bind (BinOpRCtx _ _) w w' "[Hw #Hiw]"
-                  (IHHtyped2 _ _ j (K ++ [BinOpRCtx _ _])); cbn.
+                  ('IHHtyped2 _ _ j (K ++ [BinOpRCtx _ _])); cbn.
     iDestruct "Hiv" as {n} "[% %]"; simplify_eq/=.
     iDestruct "Hiw" as {n'} "[% %]"; simplify_eq/=.
     iPvs (step_nat_bin_op _ _ j K with "* [-]") as "Hz"; eauto.
@@ -161,74 +195,71 @@ Section typed_interp.
       try destruct lt_dec; eauto.
   Qed.
 
-  Lemma typed_binary_interp_Lam Δ Γ (e e' : expr) τ1 τ2 {HΔ : ✓✓ Δ}
+  Lemma bin_log_related_Lam Δ Γ (e e' : expr) τ1 τ2 {HΔ : ✓ₚ Δ}
       (Hclosed : ∀ f, e.[iter (S (S (length Γ))) up f] = e)
       (Hclosed' : ∀ f, e'.[iter (S (S (length Γ))) up f] = e')
       (IHHtyped : Δ ∥ TArrow τ1 τ2 :: τ1 :: Γ ⊨ e ≤log≤ e' : τ2) :
     Δ ∥ Γ ⊨ Lam e ≤log≤ Lam e' : TArrow τ1 τ2.
   Proof.
-    iIntros {vvs ρ j K Hlen} "(#Hh & #Hs & #HΓ & Hj) /=".
+    iIntros {vvs ρ} "#(Hh & Hs & HΓ)"; iIntros {j K} "Hj /=".
     value_case. iExists (LamV _). iIntros "{$Hj} !".
     iLöb as "IH". iIntros {j' K' [v v'] } "[#Hiv Hv]".
+    iDestruct (interp_env_length with "HΓ") as %?.
     iApply wp_lam; auto 1 using to_of_val. iNext.
     iPvs (step_lam _ _ j' K' _ (# v') v' with "* [-]") as "Hz"; eauto.
-    asimpl.
-    specialize (IHHtyped ((LamV e.[upn 2 (env_subst (vvs.*1))],
-      LamV e'.[upn 2 (env_subst (vvs.*2))]) :: (v,v') :: vvs)); cbn in IHHtyped.
-    erewrite <- ?n_closed_subst_head_simpl_2 in IHHtyped; eauto; simpl;
-      try rewrite fmap_length; auto.
-    iApply IHHtyped; eauto 10.
+    asimpl. change (Lam ?e) with (# (LamV e)).
+    erewrite !n_closed_subst_head_simpl_2 by (rewrite ?fmap_length; eauto).
+    iApply ('IHHtyped ((_,_) :: (v,v') :: vvs)); repeat iSplit; eauto.
+    iApply interp_env_cons; iSplit; [|iApply interp_env_cons]; auto.
   Qed.
 
-  Lemma typed_binary_interp_App Δ Γ e1 e2 e1' e2' τ1 τ2 {HΔ : ✓✓ Δ}
+  Lemma bin_log_related_App Δ Γ e1 e2 e1' e2' τ1 τ2 {HΔ : ✓ₚ Δ}
       (IHHtyped1 : Δ ∥ Γ ⊨ e1 ≤log≤ e1' : TArrow τ1 τ2)
       (IHHtyped2 : Δ ∥ Γ ⊨ e2 ≤log≤ e2' : τ1) :
     Δ ∥ Γ ⊨ App e1 e2 ≤log≤ App e1' e2' :  τ2.
   Proof.
-    iIntros {vvs ρ j K Hlen} "(#Hh & #Hs & #HΓ & Hj) /=".
+    iIntros {vvs ρ} "#(Hh & Hs & HΓ)"; iIntros {j K} "Hj /=".
     smart_wp_bind (AppLCtx (e2.[env_subst (vvs.*1)])) v v' "[Hv #Hiv]"
-      (IHHtyped1 _ _ j (K ++ [(AppLCtx (e2'.[env_subst (vvs.*2)]))])); cbn.
+      ('IHHtyped1 _ _ j (K ++ [(AppLCtx (e2'.[env_subst (vvs.*2)]))])); cbn.
     smart_wp_bind (AppRCtx v) w w' "[Hw #Hiw]"
-      (IHHtyped2 _ _ j (K ++ [AppRCtx v'])); cbn.
+      ('IHHtyped2 _ _ j (K ++ [AppRCtx v'])); cbn.
     iApply ("Hiv" $! j K (w, w')); simpl; eauto.
   Qed.
 
-  Lemma typed_binary_interp_TLam Δ Γ e e' τ {HΔ : ✓✓ Δ}
+  Lemma bin_log_related_TLam Δ Γ e e' τ {HΔ : ✓ₚ Δ}
       (IHHtyped : ∀ (τi : D), (∀ vw, PersistentP (τi vw)) →
       (τi :: Δ) ∥ (subst (ren (+1)) <$> Γ) ⊨ e ≤log≤ e' : τ) :
     Δ ∥ Γ ⊨ TLam e ≤log≤ TLam e' : TForall τ.
   Proof.
-    iIntros {vvs ρ j K Hlen} "(#Hh & #Hs & #HΓ & Hj) /=".
+    iIntros {vvs ρ} "#(Hh & Hs & HΓ)"; iIntros {j K} "Hj /=".
     value_case. iExists (TLamV _).
     iIntros "{$Hj} /= !"; iIntros {τi j' K'} "% Hv /=".
     iApply wp_TLam; iNext.
-    iPvs (step_Tlam _ _ j' K' (e'.[env_subst (vvs.*2)]) with "* [-]")
-      as "Hz"; eauto.
-    iApply IHHtyped; [by rewrite fmap_length|].
-    iFrame "Hh Hs Hz". rewrite zip_with_fmap_l. by iApply context_interp_ren_S.
+    iPvs (step_Tlam _ _ j' K' (e'.[env_subst (vvs.*2)]) with "* [-]") as "Hz"; eauto.
+    iApply '(IHHtyped _ _); repeat iSplit; eauto. by iApply interp_env_ren.
   Qed.
 
-  Lemma typed_binary_interp_TApp Δ Γ e e' τ τ' {HΔ : ✓✓ Δ}
+  Lemma bin_log_related_TApp Δ Γ e e' τ τ' {HΔ : ✓ₚ Δ}
       (IHHtyped : Δ ∥ Γ ⊨ e ≤log≤ e' : TForall τ) :
     Δ ∥ Γ ⊨ TApp e ≤log≤ TApp e' : τ.[τ'/].
   Proof.
-    iIntros {vvs ρ j K Hlen} "(#Hh & #Hs & #HΓ & Hj) /=".
+    iIntros {vvs ρ} "#(Hh & Hs & HΓ)"; iIntros {j K} "Hj /=".
     smart_wp_bind (TAppCtx) v v' "[Hj #Hv]"
-      (IHHtyped _ _ j (K ++ [TAppCtx])); cbn.
+      ('IHHtyped _ _ j (K ++ [TAppCtx])); cbn.
     iApply wp_wand_r; iSplitL.
     { iApply ("Hv" $! (interp τ' Δ) with "[#] Hj"); iPureIntro; apply _. }
     iIntros {w} "Hw". iDestruct "Hw" as {w'} "[Hw #Hiw]".
     iExists _; rewrite -interp_subst; eauto.
   Qed.
 
-  Lemma typed_binary_interp_Fold Δ Γ e e' τ {HΔ : ✓✓ Δ}
+  Lemma bin_log_related_Fold Δ Γ e e' τ {HΔ : ✓ₚ Δ}
       (IHHtyped : Δ ∥ Γ ⊨ e ≤log≤ e' : τ.[(TRec τ)/]) :
     Δ ∥ Γ ⊨ Fold e ≤log≤ Fold e' : TRec τ.
   Proof.
-    iIntros {vvs ρ j K Hlen} "(#Hh & #Hs & #HΓ & Hj) /=".
+    iIntros {vvs ρ} "#(Hh & Hs & HΓ)"; iIntros {j K} "Hj /=".
     iApply (@wp_bind _ _ _ [FoldCtx]);
       iApply wp_wand_l; iSplitR;
-        [|iApply (IHHtyped _ _ j (K ++ [FoldCtx]));
+        [|iApply ('IHHtyped _ _ j (K ++ [FoldCtx]));
           rewrite ?fill_app; simpl; repeat iSplitR; trivial].
     iIntros {v}; iDestruct 1 as {w} "[Hv #Hiv]"; rewrite fill_app.
     value_case. iExists (FoldV w); iFrame "Hv".
@@ -236,14 +267,14 @@ Section typed_interp.
     iAlways; iExists (_, _); eauto.
   Qed.
 
-  Lemma typed_binary_interp_Unfold Δ Γ e e' τ {HΔ : ✓✓ Δ}
+  Lemma bin_log_related_Unfold Δ Γ e e' τ {HΔ : ✓ₚ Δ}
       (IHHtyped : Δ ∥ Γ ⊨ e ≤log≤ e' : TRec τ) :
     Δ ∥ Γ ⊨ Unfold e ≤log≤ Unfold e' : τ.[(TRec τ)/].
   Proof.
-    iIntros {vvs ρ j K Hlen} "(#Hh & #Hs & #HΓ & Hj) /=".
+    iIntros {vvs ρ} "#(Hh & Hs & HΓ)"; iIntros {j K} "Hj /=".
     iApply (@wp_bind _ _ _ [UnfoldCtx]);
       iApply wp_wand_l; iSplitR;
-        [|iApply (IHHtyped _ _ j (K ++ [UnfoldCtx]));
+        [|iApply ('IHHtyped _ _ j (K ++ [UnfoldCtx]));
           rewrite ?fill_app; simpl; repeat iSplitR; trivial].
     iIntros {v}. iDestruct 1 as {v'} "[Hw #Hiw]"; rewrite fill_app.
     rewrite /= fixpoint_unfold /=.
@@ -254,23 +285,23 @@ Section typed_interp.
     iNext; iPvsIntro; iExists _; iFrame "Hz". by rewrite -interp_subst.
   Qed.
 
-  Lemma typed_binary_interp_Fork Δ Γ e e' {HΔ : ✓✓ Δ}
+  Lemma bin_log_related_Fork Δ Γ e e' {HΔ : ✓ₚ Δ}
       (IHHtyped : Δ ∥ Γ ⊨ e ≤log≤ e' : TUnit) :
     Δ ∥ Γ ⊨ Fork e ≤log≤ Fork e' : TUnit.
   Proof.
-    iIntros {vvs ρ j K Hlen} "(#Hh & #Hs & #HΓ & Hj) /=".
+    iIntros {vvs ρ} "#(Hh & Hs & HΓ)"; iIntros {j K} "Hj /=".
     iPvs (step_fork _ _ j K with "* [-]") as {j'} "[Hj Hj']"; eauto.
     iApply wp_fork; iNext; iSplitL "Hj".
     - iExists UnitV; eauto.
-    - iApply wp_wand_l; iSplitR; [|iApply (IHHtyped _ _ _ [])]; eauto.
+    - iApply wp_wand_l; iSplitR; [|iApply ('IHHtyped _ _ _ [])]; eauto.
   Qed.
 
-  Lemma typed_binary_interp_Alloc Δ Γ e e' τ {HΔ : ✓✓ Δ}
+  Lemma bin_log_related_Alloc Δ Γ e e' τ {HΔ : ✓ₚ Δ}
       (IHHtyped : Δ ∥ Γ ⊨ e ≤log≤ e' : τ) :
     Δ ∥ Γ ⊨ Alloc e ≤log≤ Alloc e' : Tref τ.
   Proof.
-    iIntros {vvs ρ j K Hlen} "(#Hh & #Hs & #HΓ & Hj) /=".
-    smart_wp_bind (AllocCtx) v v' "[Hv #Hiv]" (IHHtyped _ _ j (K ++ [AllocCtx])).
+    iIntros {vvs ρ} "#(Hh & Hs & HΓ)"; iIntros {j K} "Hj /=".
+    smart_wp_bind (AllocCtx) v v' "[Hv #Hiv]" ('IHHtyped _ _ j (K ++ [AllocCtx])).
     iPvs (step_alloc _ _ j K (# v') v' with "* [-]") as {l'} "[Hj Hl]"; eauto.
     iApply wp_alloc; auto.
     iIntros "{$Hh} >"; iIntros {l} "Hl'".
@@ -280,12 +311,12 @@ Section typed_interp.
     iPvsIntro; iExists (LocV l'). iFrame "Hj". iExists (l, l'); eauto.
   Qed.
 
-  Lemma typed_binary_interp_Load Δ Γ e e' τ {HΔ : ✓✓ Δ}
+  Lemma bin_log_related_Load Δ Γ e e' τ {HΔ : ✓ₚ Δ}
       (IHHtyped : Δ ∥ Γ ⊨ e ≤log≤ e' : (Tref τ)) :
     Δ ∥ Γ ⊨ Load e ≤log≤ Load e' : τ.
   Proof.
-    iIntros {vvs ρ j K Hlen} "(#Hh & #Hs & #HΓ & Hj) /=".
-    smart_wp_bind (LoadCtx) v v' "[Hv #Hiv]" (IHHtyped _ _ j (K ++ [LoadCtx])).
+    iIntros {vvs ρ} "#(Hh & Hs & HΓ)"; iIntros {j K} "Hj /=".
+    smart_wp_bind (LoadCtx) v v' "[Hv #Hiv]" ('IHHtyped _ _ j (K ++ [LoadCtx])).
     iDestruct "Hiv" as { [l l'] } "[% Hinv]"; simplify_eq/=.
     iInv (logN .@ (l,l')) as { [w w'] } "[Hw1 [Hw2 #Hw]]"; simpl.
     iTimeless "Hw2".
@@ -297,16 +328,16 @@ Section typed_interp.
     - iExists w'; by iFrame.
   Qed.
 
-  Lemma typed_binary_interp_Store Δ Γ e1 e2 e1' e2' τ {HΔ : ✓✓ Δ}
+  Lemma bin_log_related_Store Δ Γ e1 e2 e1' e2' τ {HΔ : ✓ₚ Δ}
       (IHHtyped1 : Δ ∥ Γ ⊨ e1 ≤log≤ e1' : (Tref τ))
       (IHHtyped2 : Δ ∥ Γ ⊨ e2 ≤log≤ e2' : τ) :
     Δ ∥ Γ ⊨ Store e1 e2 ≤log≤ Store e1' e2' : TUnit.
   Proof.
-    iIntros {vvs ρ j K Hlen} "(#Hh & #Hs & #HΓ & Hj) /=".
+    iIntros {vvs ρ} "#(Hh & Hs & HΓ)"; iIntros {j K} "Hj /=".
     smart_wp_bind (StoreLCtx _) v v' "[Hv #Hiv]"
-      (IHHtyped1 _ _ j (K ++ [StoreLCtx _])).
+      ('IHHtyped1 _ _ j (K ++ [StoreLCtx _])).
     smart_wp_bind (StoreRCtx _) w w' "[Hw #Hiw]"
-      (IHHtyped2 _ _ j (K ++ [StoreRCtx _])).
+      ('IHHtyped2 _ _ j (K ++ [StoreRCtx _])).
     iDestruct "Hiv" as { [l l'] } "[% Hinv]"; simplify_eq/=.
     iInv (logN .@ (l,l')) as { [v v'] } "[Hv1 [Hv2 #Hv]]".
     { eapply bool_decide_spec; eauto using to_of_val. }
@@ -319,20 +350,20 @@ Section typed_interp.
     - iExists UnitV; iFrame; auto.
   Qed.
 
-  Lemma typed_binary_interp_CAS Δ Γ e1 e2 e3 e1' e2' e3' τ {HΔ : ✓✓ Δ}
+  Lemma bin_log_related_CAS Δ Γ e1 e2 e3 e1' e2' e3' τ {HΔ : ✓ₚ Δ}
       (HEqτ : EqType τ)
       (IHHtyped1 : Δ ∥ Γ ⊨ e1 ≤log≤ e1' : Tref τ)
       (IHHtyped2 : Δ ∥ Γ ⊨ e2 ≤log≤ e2' : τ)
       (IHHtyped3 : Δ ∥ Γ ⊨ e3 ≤log≤ e3' : τ) :
     Δ ∥ Γ ⊨ CAS e1 e2 e3 ≤log≤ CAS e1' e2' e3' : TBool.
   Proof.
-    iIntros {vvs ρ j K Hlen} "(#Hh & #Hs & #HΓ & Hj) /=".
+    iIntros {vvs ρ} "#(Hh & Hs & HΓ)"; iIntros {j K} "Hj /=".
     smart_wp_bind (CasLCtx _ _) v v' "[Hv #Hiv]"
-      (IHHtyped1 _ _ j (K ++ [CasLCtx _ _])).
+      ('IHHtyped1 _ _ j (K ++ [CasLCtx _ _])).
     smart_wp_bind (CasMCtx _ _) w w' "[Hw #Hiw]"
-      (IHHtyped2 _ _ j (K ++ [CasMCtx _ _])).
+      ('IHHtyped2 _ _ j (K ++ [CasMCtx _ _])).
     smart_wp_bind (CasRCtx _ _) u u' "[Hu #Hiu]"
-      (IHHtyped3 _ _ j (K ++ [CasRCtx _ _])).
+      ('IHHtyped3 _ _ j (K ++ [CasRCtx _ _])).
     iDestruct "Hiv" as { [l l'] } "[% Hinv]"; simplify_eq/=.
     iInv (logN .@ (l,l')) as { [v v'] } "[Hv1 [Hv2 #Hv]]".
     { eapply bool_decide_spec; eauto 10 using to_of_val. }
@@ -356,44 +387,34 @@ Section typed_interp.
       + iExists (♭v false); eauto.
   Qed.
 
-  Lemma typed_binary_interp Δ Γ e τ {HΔ : ctx_PersistentP Δ} :
+  Theorem binary_fundamental Δ Γ e τ {HΔ : ✓ₚ Δ} :
     Γ ⊢ₜ e : τ → Δ ∥ Γ ⊨ e ≤log≤ e : τ.
   Proof.
     intros Htyped; revert Δ HΔ; induction Htyped; intros Δ HΔ.
-    - iIntros {vvs ρ j K Hlen} "(#Hh & #Hs & #HΓ & Hj) /=".
-      destruct (lookup_lt_is_Some_2 vvs x) as [[v v'] Hv].
-      { by rewrite -Hlen; apply lookup_lt_Some with τ. }
-      rewrite /env_subst !list_lookup_fmap Hv /=. value_case.
-      iExists _; iFrame "Hj".
-      iApply (big_and_elem_of with "HΓ").
-      apply elem_of_list_lookup_2 with x.
-      rewrite lookup_zip_with; by simplify_option_eq.
-    - iIntros {vvs ρ j K Hlen} "(#Hh & #Hs & #HΓ & Hj) /=".
-      value_case. iExists UnitV; eauto.
-    - iIntros {vvs ρ j K Hlen} "(#Hh & #Hs & #HΓ & Hj) /=".
-      value_case. iExists (♯v _); eauto.
-    - iIntros {vvs ρ j K Hlen} "(#Hh & #Hs & #HΓ & Hj) /=".
-      value_case. iExists (♭v _); eauto.
-    - apply typed_binary_interp_nat_bin_op; eauto.
-    - apply typed_binary_interp_Pair; eauto.
-    - eapply typed_binary_interp_Fst; eauto.
-    - eapply typed_binary_interp_Snd; eauto.
-    - eapply typed_binary_interp_InjL; eauto.
-    - eapply typed_binary_interp_InjR; eauto.
-    - eapply typed_binary_interp_Case; eauto;
+    - by apply bin_log_related_Var.
+    - by apply bin_log_related_Unit.
+    - by apply bin_log_related_Nat.
+    - by apply bin_log_related_Bool.
+    - apply bin_log_related_nat_bin_op; eauto.
+    - apply bin_log_related_Pair; eauto.
+    - eapply bin_log_related_Fst; eauto.
+    - eapply bin_log_related_Snd; eauto.
+    - eapply bin_log_related_InjL; eauto.
+    - eapply bin_log_related_InjR; eauto.
+    - eapply bin_log_related_Case; eauto;
         match goal with H : _ |- _ => eapply (typed_n_closed _ _ _ H) end.
-    - eapply typed_binary_interp_If; eauto.
-    - eapply typed_binary_interp_Lam; eauto;
+    - eapply bin_log_related_If; eauto.
+    - eapply bin_log_related_Lam; eauto;
         match goal with H : _ |- _ => eapply (typed_n_closed _ _ _ H) end.
-    - eapply typed_binary_interp_App; eauto.
-    - eapply typed_binary_interp_TLam; eauto with typeclass_instances.
-    - eapply typed_binary_interp_TApp; eauto.
-    - eapply typed_binary_interp_Fold; eauto.
-    - eapply typed_binary_interp_Unfold; eauto.
-    - eapply typed_binary_interp_Fork; eauto.
-    - eapply typed_binary_interp_Alloc; eauto.
-    - eapply typed_binary_interp_Load; eauto.
-    - eapply typed_binary_interp_Store; eauto.
-    - eapply typed_binary_interp_CAS; eauto.
+    - eapply bin_log_related_App; eauto.
+    - eapply bin_log_related_TLam; eauto with typeclass_instances.
+    - eapply bin_log_related_TApp; eauto.
+    - eapply bin_log_related_Fold; eauto.
+    - eapply bin_log_related_Unfold; eauto.
+    - eapply bin_log_related_Fork; eauto.
+    - eapply bin_log_related_Alloc; eauto.
+    - eapply bin_log_related_Load; eauto.
+    - eapply bin_log_related_Store; eauto.
+    - eapply bin_log_related_CAS; eauto.
   Qed.
-End typed_interp.
+End fundamental.
