stlc/logrel.v
@@ -8,13 +8,19 @@ Context {Σ : iFunctor}.
 Fixpoint interp (τ : type) (w : val) : iProp lang Σ :=
   match τ with
   | TUnit => w = UnitV
-  | TProd τ1 τ2 => ∃ w1 w2, w = PairV w1 w2 ∧ interp τ1 w1 ∧ interp τ2 w2
+  | TProd τ1 τ2 => ∃ w1 w2, w = PairV w1 w2 ∧ ⟦ τ1 ⟧ w1 ∧ ⟦ τ2 ⟧ w2
   | TSum τ1 τ2 =>
-     (∃ w1, w = InjLV w1 ∧ interp τ1 w1) ∨ (∃ w2, w = InjRV w2 ∧ interp τ2 w2)
-  | TArrow τ1 τ2 =>
-     □ ∀ v, interp τ1 v → WP App (of_val w) (of_val v) {{ interp τ2 }}
-  end%I.
+     (∃ w1, w = InjLV w1 ∧ ⟦ τ1 ⟧ w1) ∨ (∃ w2, w = InjRV w2 ∧ ⟦ τ2 ⟧ w2)
+  | TArrow τ1 τ2 => □ ∀ v, ⟦ τ1 ⟧ v → WP App (# w) (# v) {{ ⟦ τ2 ⟧ }}
+  end%I
+where "⟦ τ ⟧" := (interp τ).
 
-Global Instance interp_persistent τ v : PersistentP (interp τ v).
+Definition interp_expr (τ : type) (e : expr) : iProp lang Σ :=
+  WP e {{ ⟦ τ ⟧ }}%I.
+
+Global Instance interp_persistent τ v : PersistentP (⟦ τ ⟧ v).
 Proof. revert v; induction τ=> v /=; apply _. Qed.
 End logrel.
+
+Notation "⟦ τ ⟧" := (interp τ).
+Notation "⟦ τ ⟧ₑ" := (interp_expr τ).
